Frama-C added similar benchmarks.

Frama-C/append.c
@@ -1,0 +1,62 @@
+#include <stdio.h>
+#include <stdlib.h>
+#include <string.h>
+
+// Append a single item onto the end of the array
+/*@
+  @ requires len >= 0;
+  @ requires \valid( items+ (0..len-1) );
+  @ assigns items+ (0..len-1);
+  @ ensures \valid( items+ (0..len) );
+  @ ensures \forall integer k; 0 <= k < len ==> \result[k] == \old(items[k]);
+  @ ensures items[len] == item || items == \null;
+  @*/
+int* append(int* items, const size_t len, const int item)
+{
+  // The goal is to implement, specify and verify this function!
+  int *temp = items;
+  items = malloc( (len + 1) * sizeof(int) );
+  if ( items == NULL )
+  {
+     fprintf( stderr, "append: Out Of Memory\n" );
+     free( items );
+     exit(1);
+  }
+  //@ assume \valid( items+ (0..len) );
+  memcpy( items, temp, len * sizeof(int) );
+  free( temp );
+  //@ assert items != \null;
+  items[len] = item;
+  return items;
+}
+//@ assigns \nothing;
+void fillarr( int* items, const size_t len )
+{
+  for ( int i = 0; i < len; ++i )
+    items[i] = i;
+}
+//@ assigns \nothing;
+void printarr( int* items, const size_t len )
+{
+  printf( "array = [ " );
+  for(int i = 0; i < len - 1; i++)
+    printf( "%d ,", items[i] );
+  printf( len > 0 ? "%d ]\n" : "]\n", items[len - 1] );
+}
+
+int main()
+{
+  int len = 15;
+  int* arr = malloc( len * sizeof(int) );
+  fillarr( arr, len );
+
+  printarr( arr, len );
+
+  arr = append( arr, len, len );
+
+  printarr( arr, len + 1 );
+
+  free( arr );
+  return 0;
+}
+
