Frama-C/copy.c
@@ -1,0 +1,62 @@
+#include <stdio.h>
+#include <stdlib.h>
+#include <string.h>
+
+// starting points in both arrays cannot be negative
+//@ requires sStart >= 0 && dStart >= 0 && range > 0;
+// Source array must contain enough elements to be copied
+//@ requires \length(src) >= sStart + range;
+// Destination array must have enough space for copied elements
+//@ requires \length(dest) >= dStart + range;
+//@ assigns dest+ (dStart..dStart + range - 1);
+// Result is same size as dest
+//@ ensures \length(\result) == \length(dest);
+// All elements before copied region are same
+//@ ensures forall integer k; 0 <= k < dStart ==> r[k] == dest[k];
+// All elements in copied region match src
+//@ ensures forall integer k; 0 <= k < range ==> r[dStart + k] == src[sStart + k];
+// All elements above copied region are same
+//@ ensures forall integer k; dStart + range <= k < \length(dest) ==> r[k] == dest[k];
+
+void copy( const int src[], const unsigned int sStart
+              , int dest[], const unsigned int dStart, const size_t range )
+{
+  unsigned int i = 0;
+  /*@loop invariant 0 <= i where i <= len
+    @loop invariant \length(dest) == \length(\old(dest)) */
+    // all items are still the same before dStart index
+  /*@loop invariant forall k integer; 0 <= k < dStart ==> dest[k] == odest[k]; */
+    // all items after dStart index are still the same
+  /*@loop invariant forall integer k; (dStart + len) <= k < |dest| ==> dest[k] == odest[k]; */
+    // inbetween items are copied from src
+  /*@loop invariant forall integer k, j;
+        sStart <= k < sStart + i, dStart <= j < dStart + i ==> src[k] == dest[j]; */
+  while( i < range )
+  {
+      dest[dStart + i] = src[sStart + i];
+      ++i;
+  }
+}
+
+void fillarr( int* items, size_t len, unsigned int from )
+{
+  for ( int i = 0; i < len; ++i )
+    items[i] = i + from;
+}
+
+void printarr( int* items, size_t len )
+{
+  printf( "array = [ " );
+  for(int i = 0; i < len - 1; i++)
+    printf( "%d ,", items[i] );
+  printf( len > 0 ? "%d ]\n" : "]\n", items[len - 1] );
+}
+
+int main()
+{
+  int src[] = { 6, 7, 8, 9, 10 };
+  int* res = malloc( 5 * sizeof(int) );
+  fillarr( res, 5, 1 );
+  copy( src, 1, res, 1, 3 );
+  printarr( res, 5 );
+}
