Frama-C/find.c
@@ -1,0 +1,43 @@
+#include <stdio.h>
+#include <stdlib.h>
+#include <string.h>
+
+//requires len < |arr|
+//// arr is an ordered array
+//requires all { k in 0..len - 1 | arr[k] <= arr[k + 1] }
+//// return value should not exceed len
+//ensures r <= len
+//// index of place of insertion is returned
+//ensures all { k in 0..r | arr[k] <  val }
+
+unsigned int findIns(int arr[], int val, unsigned int len)
+{
+  unsigned int i = 0;
+
+  //@ where all { k in 0..i | arr[k] < val }
+  //@ where i <= len
+  while ( i < len )
+  {
+    if ( arr[i] >= val )
+    { //@ assert all { k in i..len | arr[k] >= val }
+      return i;
+    }
+    ++i;
+  }
+  return i;
+}
+
+void printarr( int* items, int len )
+{
+  printf( "array = [ " );
+  for(int i = 0; i < len - 1; i++)
+    printf( "%d ,", items[i] );
+  printf( len > 0 ? "%d ]\n" : "]\n", items[len - 1] );
+}
+
+int main()
+{
+    int arr[] = { 1,2,3,4,5 };
+    findIns( arr, 3, 5 );
+    printarr( arr, 5 );
+}
