Frama-C/insert.c
@@ -1,0 +1,63 @@
+#include <stdio.h>
+#include <stdlib.h>
+#include <string.h>
+
+// This function should insert the item at the given
+// index from the items array.  The resulting array is of
+// course one element longer in length.
+//  requires index < len
+//  requires len > 0
+//  ensures |r| == len + 1
+//  ensures all { k in 0..index | r[k] == items[k] }
+//  ensures r[index] == item
+//  ensures all { k in index..len | r[k] == items[k - 1] }
+void insert( int items[], unsigned int len, int item, unsigned int index )
+{
+  // length of the new array
+  unsigned int newlen = len + 1;
+  unsigned int i = len;
+    int *temp = items;
+  items = realloc( items, newlen * sizeof(int) );
+  if ( items == NULL )
+  {
+    items = malloc( newlen * sizeof(int) );
+    if ( items == NULL )
+    {
+      fprintf( stderr, "append: Out Of Memory\n" );
+      free( items );
+      exit(1);
+    }
+    memcpy( items, temp, len * sizeof(int) );
+    free( temp );
+  }
+
+  while ( index < i )
+  {
+    items[i] = items[i - 1];
+    --i;
+  }
+  items[i] = item;
+}
+
+void fillarr( int* items, int len )
+{
+  for ( int i = 0; i < len; ++i )
+    items[i] = i;
+}
+
+void printarr( int* items, int len )
+{
+  printf( "array = [ " );
+  for(int i = 0; i < len - 1; i++)
+    printf( "%d ,", items[i] );
+  printf( len > 0 ? "%d ]\n" : "]\n", items[len - 1] );
+}
+
+int main()
+{
+    int* res = malloc( 5 * sizeof(int) );
+    fillarr( res, 5 );
+    printarr( res, 5 );
+    insert( res, 5, 1, 3 );
+    printarr( res, 6 );
+}
