Frama-C/lastIndexOf.c
@@ -1,0 +1,48 @@
+#include <stdio.h>
+#include <stdlib.h>
+#include <string.h>
+
+// If result is positive, element at that position must match item
+//@ ensures r >= 0 ==> items[r] == item
+// If result is positive, no element at greater position matches item
+//@ ensures r >= 0 ==> all { x in (r + 1)..|items| | items[x] != item }
+// If result is negative, no element matches item
+//@ ensures r < 0 ==> no { x in 0..|items| | items[x] == item }:
+int lastIndexOf( int items[], const unsigned int len, const int item )
+{
+    int i = len;
+    // i is decreasing and no element at greater position matches item
+    //@    where i <= |items|;
+    //@    where no { x in i..|items| | items[x] == item };
+    while ( i > 0 )
+    {
+        --i;
+        if ( items[i] == item )
+            return i;
+    }
+    // didn't find item in entire list
+    return -1;
+}
+
+void fillarr( int* items, int len )
+{
+  for ( int i = 0; i < len; ++i )
+    items[i] = i;
+}
+
+void printarr( int* items, int len )
+{
+  printf( "array = [ " );
+  for(int i = 0; i < len - 1; i++)
+    printf( "%d ,", items[i] );
+  printf( len > 0 ? "%d ]\n" : "]\n", items[len - 1] );
+}
+
+int main()
+{
+    int len = 5;
+    int* res = malloc( len * sizeof(int) );
+    fillarr( res, len );
+    printarr( res, len );
+    printf( "last index of %d is %d", len, lastIndexOf( res, len, 3 ) );
+}
