Frama-C/palindrome.c
@@ -1,0 +1,46 @@
+#include <stdio.h>
+#include <stdlib.h>
+#include <string.h>
+
+// Result holds iff array is a palindrome :)
+//@ requires |chars| != 0
+//@ ensures r <==> all { x in 0..|chars| | chars[x] == chars[|chars| - (x + 1)] }:
+int isPalindrome(int chars[], unsigned int len )
+{
+    int i = 0;
+    int j = len;
+//@ where i + j == |chars| && i >= 0
+//@ where all { k in 0..i | chars[k] == chars[|chars| - (k+1)] }:
+  while ( i < j )
+  {
+    --j;
+    if ( chars[i] != chars[j] )
+      return 0;
+    ++i;
+  }
+  return 1;
+}
+
+void fillarr( int* items, int len )
+{
+  for ( int i = 0; i < len; ++i )
+    items[i] = i;
+}
+
+void printarr( int* items, int len )
+{
+  printf( "array = [ " );
+  for(int i = 0; i < len - 1; i++)
+    printf( "%d ,", items[i] );
+  printf( len > 0 ? "%d ]\n" : "]\n", items[len - 1] );
+}
+
+int main()
+{
+  int len = 5;
+  int* res = malloc( len * sizeof(int) );
+  fillarr( res, len );
+  printarr( res, len );
+  printf( isPalindrome( res, len ) ? " is " : " is not " );
+  printf( " a Palindrome." );
+}
