Frama-C/remove.c
@@ -1,0 +1,54 @@
+// Status: verifier "GC overhead limit exceeded"
+// This function should remove the item at the given
+// index from the items array, and return the resulting
+// array otherwise unchanged.  The resulting array is of
+// course one element shorter in length.
+/*@
+  @ requires index < len;
+  @ requires len > 0;
+  @ ensures \valid(\result+ (0..len-2) );
+  @ ensures forall integer k; 0 <= k < index ==> \result[k] == \old(items[k]);
+  @ ensures forall integer k; index <= k < (len-1) ==> r[k] == items[k + 1];
+*/
+int *remove( int items[], unsigned int len , unsigned int index)
+{
+  unsigned int newlen = len - 1;
+  unsigned int i = index;
+  int *temp = items;
+  // items before index in result are still the same
+  /*@
+    @ where 0 <= i where i <= index
+    @ where |result| == newlen
+    @ where all { k in 0..i | k < index ==> result[k] == items[k] }
+  */
+
+  /*@
+    @ where index <= i where i <= newlen
+    @ where |result| == newlen
+    @ where all { k in 0..index | result[k] == items[k] }
+    @ where all { k in index..i | result[k] == items[k + 1] }
+  */
+  while ( i < newlen )
+  // items after index in result are transposed by one place
+  {
+    items[i] = items[i + 1];
+    ++i;
+  }
+
+  items = realloc( items, (len - 1) * sizeof(int) );
+  //@ assert items == \null || \valid( items+ (0..len - 2) );
+  if ( items == NULL )
+  {
+    items = malloc( (len - 1) * sizeof(int) );
+    if ( items == NULL )
+    {
+       fprintf( stderr, "append: Out Of Memory\n" );
+       free( items );
+       exit(1);
+    }
+    memcpy( items, temp, (len - 1) * sizeof(int) );
+    free( temp );
+  }
+
+  return items;
+}
