Frama-C/search.c
@@ -1,0 +1,25 @@
+// Status: verified and compiled
+type nat is (int n) where n >= 0
+
+// A linear search over a sorted array looking for a given element.
+function search(int[] ls, int item) -> (int r)
+//////////////////////////////////////////////
+requires |ls| > 0
+// ls is an ordered array
+requires all { k in 0..|ls| - 1 | ls[k] <= ls[k + 1] }
+// if not found return index is -1
+ensures r < 0 ==> all { k in 0..|ls| | ls[k] != item }
+// if found the index is returned
+ensures r >= 0 ==> ls[r] == item
+:
+    nat i = 0
+    
+    while i < |ls|
+    where i <= |ls|
+    where all { k in 0..i | ls[k] != item }
+    :
+        if ls[i] == item:
+            return i
+        i = i + 1
+    
+    return -1
