Frama-C/strlen.c
@@ -1,0 +1,29 @@
+#include <stdio.h>
+
+// Calculate length of string
+/*@
+  @ assigns \nothing;
+  @ ensures str[\result] == '\0'; */
+unsigned int strlength( const char* str )
+{
+  unsigned int i = 0;
+  /*@ loop invariant i >= 0;
+    @ loop invariant \forall integer k; 0 <= k < i ==> str[k] != '\0'; */
+  while ( str[i] != '\0' ) ++i;
+
+  return i;
+}
+
+void printarr( const char* items )
+{
+  printf( "array = [ " );
+  printf( items );
+  printf( " ]\n" );
+}
+
+int main()
+{
+  const char* res = "ABCDEFGHIJKLMNOP";
+  printarr( res );
+  printf( " has length of %d\n", strlength( res ) );
+}
