Dafny/alt/displace.dfy
@@ -1,0 +1,28 @@
+// Status: verifies and compiles
+// rotates a region of the array by one place backward
+method displace(arr: array<int>, start: nat, len: nat)
+  modifies arr
+  requires arr != null
+  requires start + len <= arr.Length
+  //
+  ensures arr != null && arr.Length == old(arr.Length)
+  ensures forall k: nat :: k < start ==> arr[k] == old(arr[k])
+  ensures forall k: nat :: (start + len) <= k < arr.Length ==> arr[k] == old(arr[k])
+  ensures forall k :: start <= k < (start + len)
+                 ==> arr[start + (((k + 1) - start) % len)] == old(arr[k])
+{
+  var i := start + len - 2;
+  var temp := arr[start + len - 1];
+  
+  while i >= start
+    invariant start <= i <= (start + len)
+    invariant arr[..start] == old(arr[..start])
+    invariant forall k :: start <= k < i
+              ==> arr[start + (((k + 1) - start) % len)] == old(arr[k])
+    invariant arr[(start + len)..] == old(arr[(start + len)..])
+  {
+      arr[i + 1] := arr[i];
+      i := i - 1;
+  }
+  arr[start] := temp;
+}
