Dafny/alt/displace2.dfy
@@ -2,16 +2,17 @@
 // rotates a region of the array by one place forward
 method displace(arr: array<int>, start: nat, len: nat) returns (r: array<int>)
   requires arr != null
-  requires start + len <= arr.Length
+  requires start + len < arr.Length
   // returned array is the same size as input arr
   ensures r != null && r.Length == arr.Length
+  ensures start + len <= r.Length
   // elements before the start of the region are unchanged
   ensures arr[..start] == r[..start]
   // elements after the end of the rhe region are unchanged
-  ensures arr[(start + len)..] == r[(start + len)..]
+  ensures arr[(start + len + 1)..] == r[(start + len + 1)..]
   // elements in the region are skewed by one in a positive direction and wrap around
-  ensures forall k :: start <= k < (start + len)
-                 ==> r[start + (((k + 1) - start) % len)] == arr[k]
+  ensures r[start] == arr[start + len]
+  ensures forall k :: start < k < (start + len) ==> r[k + 1] == arr[k]
 {
     var i: nat := 0;
     r := new int[arr.Length];
@@ -27,11 +28,12 @@ method displace(arr: array<int>, start: nat, len: nat) returns (r: array<int>)
     i := start;
     
     while i < (start + len)
+      invariant r.Length == arr.Length
       invariant start <= i <= (start + len)
       invariant arr[..start] == r[..start]
-      invariant arr[(start + len)..] == r[(start + len)..]
-      invariant forall k :: start <= k < i
-                ==> r[start + (((k + 1) - start) % len)] == arr[k]
+      invariant arr[(start + len + 1)..] == r[(start + len + 1)..]
+      invariant forall k :: start < k < i ==> r[k + 1] == arr[k]
+      invariant i == start + len ==> r[start] == arr[start + len]
     {
         r[start + (((i + 1) - start) % len)] := arr[i];
         i := i + 1;
