Dafny/copy.dfy
@@ -4,20 +4,20 @@
 method copy( src: array<int>, sStart: nat, dest: array<int>, dStart: nat, len: nat)
     returns (r: array<int>)
   // both arrays cannot be null
-   requires dest != null && src != null
+  requires dest != null && src != null;
   // Source array must contain enough elements to be copied
-   requires src.Length >= sStart + len
+  requires src.Length >= sStart + len;
   // Destination array must have enough space for copied elements
-   requires dest.Length >= dStart + len
+  requires dest.Length >= dStart + len;
   // Result is same size as dest
-  ensures r != null
-  ensures r.Length == dest.Length
+  ensures r != null;
+  ensures r.Length == dest.Length;
   // All elements before copied region are same
-   ensures r[..dStart] == dest[..dStart]
+  ensures r[..dStart] == dest[..dStart];
   // All elements above copied region are same
-   ensures r[dStart + len..] == dest[dStart + len..]
+  ensures r[dStart + len..] == dest[dStart + len..];
   // All elements in copied region match src
-   ensures forall k: nat :: k < len ==> r[dStart + k] == src[sStart + k]
+  ensures forall k: nat :: k < len ==> r[dStart + k] == src[sStart + k];
   
 {
     if len == 0 { return dest; }
