Frama-C/displace.whiley
@@ -1,0 +1,34 @@
+// Status: causes infinite loop in verifier
+type nat is (int n) where n >= 0
+
+// rotates a region of the array by one place forward
+function displace(int[] arr, nat start, nat len) -> (int[] r)
+/////////////////////////////////////////////////////////////
+requires start + len <= |arr|
+// output array is the same size as input array
+ensures |r| == |arr|
+// all elements before the region remain the same
+ensures all { k in 0..start | r[k] == arr[k] }
+// all elements after the region remain the same
+ensures all { k in (start + len)..|arr| | r[k] == arr[k] }
+// all elements in the region are rotated by one place
+ensures all { k in start..start + len | r[k] == arr[start + (((k + 1) - start) % len)] }
+:
+  nat i = start
+  int[] result = arr
+  assert all { k in 0..|result| | result[k] == arr[k] }
+
+  while i < (start + len)
+
+  where start <= i where i <= (start + len)
+  where |result| == |arr|
+  where all { k in 0..start | result[k] == arr[k] }
+  where all { k in start..i | result[k] == arr[start + (((k + 1) - start) % len)] }
+  where all { k in (start + len)..|arr| | result[k] == arr[k] }
+  :
+      result[i] = arr[start + (((i + 1) - start) % len)]
+      i = i + 1
+
+  assert i == (start + len)
+  
+  return result
