find.whiley
@@ -1,4 +1,24 @@
-method findIns(arr: array<int>, val: int) returns (r: nat)
-{
-  
-}
+type nat is (int n) where n >= 0
+
+function findIns(int[] arr, int val, nat len) -> (nat r)
+///////////////////////////////////////////////
+requires len < |arr|
+// arr is an ordered array
+requires all { k in 0..len - 1 | arr[k] <= arr[k + 1] }
+// return value should not exceed len
+ensures r <= len
+// index of place of insertion is returned
+ensures all { k in 0..r | arr[k] <  val }
+:
+    nat i = 0
+    
+    while i < len
+
+    where i <= len
+    where all { k in 0..i | arr[k] < val }
+    :
+        if arr[i] >= val:
+            assert all { k in i..len | arr[k] >= val }
+            return i
+        i = i + 1
+    return i
